Demostrar que
=============

## a) flip (curry f) = curry (f . swap)

si
1) f :: (a,b) -> c
2) y :: a
3) x :: b


flip (curry f) x y
=  def.flip
(curry f) y x
=  def. curry
f (y,x)
=  def. swap
f (swap (x,y))
= aplicaciÃ³n de '.'
(f . swap) (x,y)
= def. curry
curry (f . swap) x y




## b) Sean i j k tales que i â‰¤ j â‰¤ k, vale
## sum f i j + sum f (j+1) k = sum f i k

sum :: (Int -> Int) -> Int -> Int -> Int
f :: Int -> Int -> [Int]
i :: Int
j :: Int
k :: Int

sum f i j + sum f (j+1) k
= def. sum
(f i) + (sum f i+1 j) + sum f (j+1) k
= def. sum
(f i) + ((f i+1) + (sum f i+1+1 j)) + sum f (j+1) k
= def. sum
(f i) + ((f i+1) + ((f i+1+1) + (sum f i+1+1+1 j))) + sum f (j+1) k
= arit.
(f i) + (f i+1) + (f i+2) + ... + (f j-1) + (sum f j j) + sum f (j+1) k
= def. sum
(f i) + (f i+1) + (f i+2) + ... + (f j-1) + (f j) + sum f (j+1) k
= def. sum
(f i) + (f i+1) + (f i+2) + ... + (f j-1) + (f j) + (f j+1) + (f j+2) + ... + (f k-1) + sum f k k
= def. sum
(f i) + (f i+1) + (f i+2) + ... + (f j-1) + (f j) + (f j+1) + (f j+2) + ... + (f k-1) + (f k)
= arit.
(f i) + (f i+1) + ... + (f k-1) + (f k)
= def. sum
(f i) + (f i+1) + ... + (f k-1) + sum f k k
= def. sum
(f i) + (f i+1) + (sum f i+2 k)
= def. sum
(f i) + (sum f i+1 k)
= def. sum
sum f i+1 k
